properties about simulation between encapsulated lts

common/CategoricalComp.v
@@ -443,6 +443,319 @@ Proof.
   - destruct Ha, Hb. congruence.
 Qed.
 
+Variable id_skel: AST.program unit unit.
+Hypothesis id_skel_order: forall sk, Linking.linkorder id_skel sk.
+
+Section ID_SEM.
+
+  Context {liA liB} (L: semantics liA liB).
+
+  (*
+  Definition id_skel: AST.program unit unit :=
+    {|
+      prog_defs := nil;
+      prog_public := nil;
+      prog_main := prog_main (skel L);
+    |}.
+  Lemma id_skel_order: Linking.linkorder id_skel (skel L).
+  Proof.
+    constructor. reflexivity.
+    repeat split. easy.
+    intros. inv H.
+  Qed.
+  *)
+
+  Definition left_comp_id :=
+    comp_semantics' (id_semantics id_skel) L (skel L).
+  Definition right_comp_id :=
+    comp_semantics' L (id_semantics id_skel) (skel L).
+
+End ID_SEM.
+
+Notation "L 'o' 1" := (right_comp_id L) (at level 15).
+Notation "1 'o' L" := (left_comp_id L) (at level 20).
+(* Notation "1 [ L ]" := (id_semantics (id_skel L)). *)
+Notation "1" := (id_semantics id_skel) : lts_scope.
+Definition normalize_sem {liA liB} (L: semantics liA liB) := 1 o L o 1.
+
+(* TODO: maybe we need to use CAT.fsim to define E.fsim *)
+
+Ltac inv_comp :=
+  match goal with
+  | [ H : at_external ((_ (comp_semantics' _ _ _)) _) _ _ |- _ ] => inv H
+  | [ H : after_external ((_ (comp_semantics' _ _ _)) _) _ _ _ |- _ ] => inv H
+  | [ H : initial_state ((_ (comp_semantics' _ _ _)) _) _ _ |- _ ] => inv H
+  | [ H : final_state ((_ (comp_semantics' _ _ _)) _) _ _ |- _ ] => inv H
+  | [ H : step ((_ (comp_semantics' _ _ _)) _) _ _ _ _ |- _ ] => inv H
+  end.
+Ltac inv_id :=
+  match goal with
+  | [ H : at_external ((_ (id_semantics _)) _) _ _ |- _ ] => inv H
+  | [ H : after_external ((_ (id_semantics _)) _) _ _ _ |- _ ] => inv H
+  | [ H : initial_state ((_ (id_semantics _)) _) _ _ |- _ ] => inv H
+  | [ H : final_state ((_ (id_semantics _)) _) _ _ |- _ ] => inv H
+  | [ H : step ((_ (id_semantics _)) _) _ _ _ _ |- _ ] => inv H
+  end.
+Ltac ese := eexists; repeat split; eauto.
+
+Module CAT.
+
+  Definition forward_simulation
+             {liA1 liA2} (ccA: callconv liA1 liA2)
+             {liB1 liB2} (ccB: callconv liB1 liB2) L1 L2 :=
+    forward_simulation ccA ccB (normalize_sem L1) (normalize_sem L2).
+
+  Section ID_PROPS.
+
+    Context {liA liB} (L: semantics liA liB).
+
+    (* TODO: notations like (st4 _ _ _ _ s1 s2 s3 s4) *)
+    Inductive lu_ms: state (1 o L o 1) -> state (1 o (1 o L o 1)) -> Prop :=
+    | lu_ms1 q:
+      lu_ms (st1 1 _ (st_q q)) (st1 1 _ (st_q q))
+    | lu_ms2 q s:
+      lu_ms (st2 1 (L o 1) (st_q q) (st1 L _ s))
+            (st2 1 (1 o L o 1) (st_q q) (st2 1 (L o 1) (st_q q) (st1 L _ s)))
+    | lu_ms3 qi s qo:
+      lu_ms (st2 1 (L o 1) (st_q qi) (st2 L 1 s (st_q qo)))
+            (st2 1 (1 o L o 1) (st_q qi) (st2 1 (L o 1) (st_q qi) (st2 L 1 s (st_q qo))))
+    | lu_ms4 qi s ro:
+      lu_ms (st2 1 (L o 1) (st_q qi) (st2 L 1 s (st_r ro)))
+            (st2 1 (1 o L o 1) (st_q qi) (st2 1 (L o 1) (st_q qi) (st2 L 1 s (st_r ro))))
+    | lu_ms5 r:
+      lu_ms (st1 1 _ (st_r r)) (st1 1 _ (st_r r)).
+
+    Hint Constructors lu_ms.
+
+    Lemma left_unit_1: forward_simulation 1 1 L (left_comp_id L).
+    Proof.
+      unfold forward_simulation, normalize_sem.
+      etransitivity. instantiate (1 := 1 o (1 o L o 1)).
+      2: {
+        eapply categorical_compose_simulation'.
+        reflexivity. apply assoc1.
+        eapply Linking.linkorder_trans. apply id_skel_order.
+        1-2: apply Linking.linkorder_refl.
+      }
+      constructor.
+      eapply Forward_simulation
+        with (fsim_order := (ltof _ (fun _ => O)))
+             (fsim_match_states := fun _ _ _ x s1 s2 => x = s1 /\ lu_ms s1 s2).
+      reflexivity. firstorder. 2: apply well_founded_ltof.
+      intros se ? [] [] Hse. clear Hse.
+      apply forward_simulation_plus;
+        unfold left_comp_id, right_comp_id in *.
+      - intros. inv H. repeat (inv_comp || inv_id). ese.
+      - intros. repeat (inv_comp || inv_id). inv H. ese.
+      - intros. repeat (inv_comp || inv_id). exists tt.
+        inv H. ese.
+        intros. repeat (inv_comp || inv_id). inv H. ese.
+      - intros * HSTEP s2 HS. inv HS.
+        + inv HSTEP; repeat (inv_comp || inv_id). ese.
+          eapply plus_two. eapply step_push; repeat constructor.
+          eapply step2. eapply step_push; repeat constructor; eauto.
+          reflexivity.
+        + inv HSTEP; repeat (inv_comp || inv_id).
+          * ese. apply plus_one.
+            apply step2. apply step2. apply step1; eassumption.
+          * ese. apply plus_one. apply step2. apply step2.
+            eapply step_push; try constructor; eauto.
+          * ese. eapply plus_two.
+            apply step2. eapply step_pop; constructor; eauto.
+            eapply step_pop; repeat constructor; eauto.
+            reflexivity.
+        + inv HSTEP; repeat (inv_comp || inv_id).
+        + inv HSTEP; repeat (inv_comp || inv_id).
+          ese. apply plus_one. apply step2. apply step2.
+          eapply step_pop; repeat constructor; eauto.
+        + inv HSTEP; repeat (inv_comp || inv_id).
+    Qed.
+
+    Definition ul_measure (s: state (1 o (1 o L o 1))) :=
+      match s with
+      | st1 _ _ (st_q _) => 1%nat
+      | st2 _ _ (st_q _) (st1 _ _ (st_q _)) => 0%nat
+      | st2 _ _ (st_q _) (st1 _ _ (st_r _)) => 1%nat
+      | st1 _ _ (st_r _) => 0%nat
+      | _ => 0%nat
+      end.
+    Inductive ul_ms: state (1 o (1 o L o 1)) -> state (1 o L o 1) -> Prop :=
+    | ul_ms1 q:
+      ul_ms (st1 1 _ (st_q q)) (st1 1 _ (st_q q))
+    | ul_ms1' q:
+      ul_ms (st2 1 (1 o L o 1) (st_q q) (st1 1 _ (st_q q))) (st1 1 _ (st_q q))
+    | ul_ms2 q s:
+      ul_ms (st2 1 (1 o L o 1) (st_q q) (st2 1 (L o 1) (st_q q) (st1 L _ s)))
+            (st2 1 (L o 1) (st_q q) (st1 L _ s))
+    | ul_ms3 qi s qo:
+      ul_ms (st2 1 (1 o L o 1) (st_q qi) (st2 1 (L o 1) (st_q qi) (st2 L 1 s (st_q qo))))
+             (st2 1 (L o 1) (st_q qi) (st2 L 1 s (st_q qo)))
+    | ul_ms4 qi s ro:
+      ul_ms (st2 1 (1 o L o 1) (st_q qi) (st2 1 (L o 1) (st_q qi) (st2 L 1 s (st_r ro))))
+            (st2 1 (L o 1) (st_q qi) (st2 L 1 s (st_r ro)))
+    | ul_ms5 r:
+      ul_ms (st1 1 _ (st_r r)) (st1 1 _ (st_r r))
+    | ul_ms5' q r:
+      ul_ms (st2 1 (1 o L o 1) (st_q q) (st1 1 _ (st_r r))) (st1 1 _ (st_r r)).
+    Hint Constructors ul_ms.
+
+    Lemma left_unit_2: forward_simulation 1 1 (left_comp_id L) L.
+    Proof.
+      unfold forward_simulation, normalize_sem.
+      etransitivity. instantiate (1 := 1 o (1 o L o 1)).
+      {
+        eapply categorical_compose_simulation'.
+        reflexivity. apply assoc2.
+        eapply Linking.linkorder_trans. apply id_skel_order.
+        1-2: apply Linking.linkorder_refl.
+      }
+      constructor.
+      eapply Forward_simulation
+        with (fsim_order := (ltof _ ul_measure))
+             (fsim_match_states := fun _ _ _ i s1 s2 => i = s1 /\ ul_ms s1 s2).
+      reflexivity. firstorder. 2: apply well_founded_ltof.
+      intros se ? [] [] Hse.
+      eapply forward_simulation_opt;
+        unfold left_comp_id, right_comp_id in *.
+      - intros. inv H. repeat (inv_comp || inv_id). ese.
+      - intros. repeat (inv_comp || inv_id). inv H. ese.
+      - intros. repeat (inv_comp || inv_id). inv H. exists tt. ese.
+        intros. repeat (inv_comp || inv_id). inv H. ese.
+      - intros * HSTEP s HS. inv HS.
+        + inv HSTEP; repeat (inv_comp || inv_id).
+          right. repeat split; eauto.
+        + inv HSTEP; repeat (inv_comp || inv_id).
+          left. ese. eapply step_push; constructor; eauto.
+        + inv HSTEP; repeat (inv_comp || inv_id).
+          * left. ese. apply step2. apply step1. assumption.
+          * left. ese. apply step2.
+            eapply step_push; repeat constructor; eauto.
+          * left. ese.
+            eapply step_pop; repeat constructor; eauto.
+        + inv HSTEP; repeat (inv_comp || inv_id).
+        + inv HSTEP; repeat (inv_comp || inv_id).
+          left. ese.
+          apply step2. eapply step_pop; repeat constructor; eauto.
+        + inv HSTEP; repeat (inv_comp || inv_id).
+        + inv HSTEP; repeat (inv_comp || inv_id).
+          right. cbn. repeat split; eauto.
+    Qed.
+
+    Inductive ru_ms: state (1 o L o 1) -> state (1 o (L o 1) o 1) -> Prop :=
+    | ru_ms1 q:
+      ru_ms (st1 1 _ (st_q q)) (st1 1 _ (st_q q))
+    | ru_ms2 q s:
+      ru_ms (st2 1 (L o 1) (st_q q) (st1 L _ s))
+            (st2 1 ((L o 1) o 1) (st_q q) (st1 (L o 1) _ (st1 L _ s)))
+    | ru_ms3 qi s qo:
+      ru_ms (st2 1 (L o 1) (st_q qi) (st2 L 1 s (st_q qo)))
+            (st2 1 ((L o 1) o 1) (st_q qi) (st2 (L o 1) 1 (st2 L 1 s (st_q qo)) (st_q qo)))
+    | ru_ms4 qi s qo ro:
+      ru_ms (st2 1 (L o 1) (st_q qi) (st2 L 1 s (st_r ro)))
+            (st2 1 ((L o 1) o 1) (st_q qi) (st2 (L o 1) 1 (st2 L 1 s (st_q qo)) (st_r ro)))
+    | ru_ms5 r:
+      ru_ms (st1 1 _ (st_r r)) (st1 1 _ (st_r r)).
+    Hint Constructors ru_ms.
+
+    Lemma right_unit_1: forward_simulation 1 1 L (right_comp_id L).
+    Proof.
+      unfold forward_simulation, normalize_sem.
+      constructor.
+      eapply Forward_simulation with (ltof _ (fun _ => O))
+                                     (fun _ _ _ x s1 s2 => x = s1 /\ ru_ms s1 s2).
+      reflexivity. firstorder. 2: apply well_founded_ltof.
+      intros se ? [] [] Hse. clear Hse.
+      apply forward_simulation_plus;
+        unfold left_comp_id, right_comp_id in *.
+      - intros. inv H. repeat (inv_comp || inv_id). ese.
+      - intros. repeat (inv_comp || inv_id). inv H. ese.
+      - intros. repeat (inv_comp || inv_id). inv H. exists tt. ese.
+        intros. repeat (inv_comp || inv_id). inv H. ese.
+      - intros * HSTEP s HS. inv HS.
+        + inv HSTEP; repeat (inv_comp || inv_id). ese.
+          apply plus_one. eapply step_push; repeat constructor; eauto.
+        + inv HSTEP; repeat (inv_comp || inv_id).
+          * ese. apply plus_one.
+            apply step2. apply step1. apply step1. assumption.
+          * ese. eapply plus_two.
+            apply step2. apply step1. eapply step_push; eauto. constructor.
+            apply step2. eapply step_push; repeat constructor.
+            reflexivity.
+          * ese. apply plus_one.
+            eapply step_pop; repeat constructor. assumption.
+        + inv HSTEP; repeat (inv_comp || inv_id).
+        + inv HSTEP; repeat (inv_comp || inv_id).
+          ese. eapply plus_two.
+          apply step2. eapply step_pop; repeat constructor.
+          apply step2. apply step1. eapply step_pop; try constructor; eauto.
+          reflexivity.
+        + inv HSTEP; repeat (inv_comp || inv_id).
+    Qed.
+
+    Definition ur_measure (s: state (1 o (L o 1) o 1)) :=
+      match s with
+      | st2 _ _ (st_q qi) (st1 _ _ (st2 _ _ s (st_q qo))) => 1%nat
+      | st2 _ _ (st_q qi) (st2 _ _ (st2 _ _ s (st_q qo)) (st_r ro)) => 1%nat
+      | _ => 0%nat
+      end.
+    Inductive ur_ms: state (1 o (L o 1) o 1) -> state (1 o L o 1) -> Prop :=
+    | ur_ms1 q:
+      ur_ms (st1 1 _ (st_q q)) (st1 1 _ (st_q q))
+    | ur_ms2 q s:
+      ur_ms (st2 1 ((L o 1) o 1) (st_q q) (st1 (L o 1) _ (st1 L _ s)))
+            (st2 1 (L o 1) (st_q q) (st1 L _ s))
+    | ur_ms3 qi s qo:
+      ur_ms (st2 1 ((L o 1) o 1) (st_q qi) (st2 (L o 1) 1 (st2 L 1 s (st_q qo)) (st_q qo)))
+            (st2 1 (L o 1) (st_q qi) (st2 L 1 s (st_q qo)))
+    | ur_ms3' qi s qo:
+      ur_ms (st2 1 ((L o 1) o 1) (st_q qi) (st1 (L o 1) _ (st2 L 1 s (st_q qo))))
+            (st2 1 (L o 1) (st_q qi) (st2 L 1 s (st_q qo)))
+    | ur_ms4 qi s qo ro:
+      ur_ms (st2 1 ((L o 1) o 1) (st_q qi) (st2 (L o 1) 1 (st2 L 1 s (st_q qo)) (st_r ro)))
+            (st2 1 (L o 1) (st_q qi) (st2 L 1 s (st_r ro)))
+    | ur_ms4' qi s ro:
+      ur_ms (st2 1 ((L o 1) o 1) (st_q qi) (st1 (L o 1) _ (st2 L 1 s (st_r ro))))
+            (st2 1 (L o 1) (st_q qi) (st2 L 1 s (st_r ro)))
+    | ur_ms5 r:
+      ur_ms (st1 1 _ (st_r r)) (st1 1 _ (st_r r)).
+    Hint Constructors ur_ms.
+
+    Lemma right_unit_2: forward_simulation 1 1 (right_comp_id L) L.
+    Proof.
+      constructor.
+      eapply Forward_simulation
+        with (fsim_order := (ltof _ ur_measure))
+             (fsim_match_states := fun _ _ _ i s1 s2 => i = s1 /\ ur_ms s1 s2).
+      reflexivity. firstorder. 2: apply well_founded_ltof.
+      intros se ? [] [] Hse. clear Hse.
+      eapply forward_simulation_opt;
+        unfold left_comp_id, right_comp_id in *.
+      - intros. inv H. repeat (inv_comp || inv_id). ese.
+      - intros. repeat (inv_comp || inv_id). inv H. ese.
+      - intros. repeat (inv_comp || inv_id). inv H. exists tt. ese.
+        intros. repeat (inv_comp || inv_id). inv H. ese.
+      - intros * HSTEP s HS. inv HS.
+        + inv HSTEP; repeat (inv_comp || inv_id).
+          left. ese. eapply step_push; constructor; eauto.
+        + inv HSTEP; repeat (inv_comp || inv_id).
+          * left. ese. apply step2. apply step1. assumption.
+          * left. ese. apply step2. eapply step_push; eauto. constructor.
+          * left. ese. eapply step_pop; constructor. assumption.
+        + inv HSTEP; repeat (inv_comp || inv_id).
+        + inv HSTEP; repeat (inv_comp || inv_id).
+          right. repeat split; eauto.
+        + inv HSTEP; repeat (inv_comp || inv_id).
+          right. repeat split; eauto.
+        + inv HSTEP; repeat (inv_comp || inv_id).
+          left. ese. apply step2. eapply step_pop; try constructor; eauto.
+        + inv HSTEP; repeat (inv_comp || inv_id).
+    Qed.
+
+  End ID_PROPS.
+  (* These properties are then lifted to ST.fsim *)
+
+End CAT.
+
 Section APPROX.
   Context {li} (L1 L2: semantics li li).
   Context `{!CategoricalLinkable L1 L2}
@@ -688,3 +1001,171 @@ Section HCOMP_IDENTITY.
   Qed.
 
 End HCOMP_IDENTITY.
+
+Generalizable All Variables.
+
+Section NORMALIZE_COMP.
+
+  Context `(L1: semantics liB liC) `(L2: semantics liA liB).
+  Variable sk: AST.program unit unit.
+
+  Inductive nc_ms: state (comp_semantics' L1 L2 sk) ->
+                   state (comp_semantics' (L1 o 1) (1 o L2) sk) -> Prop :=
+  | nc_ms1 s:
+    nc_ms (st1 L1 _ s)
+          (st1 (L1 o 1) _ (st1 L1 _ s))
+  | nc_ms2 s1 s2 q:
+    nc_ms (st2 L1 L2 s1 s2)
+          (st2 (L1 o 1) (1 o L2) (st2 L1 1 s1 (st_q q)) (st2 1 L2 (st_q q) s2)).
+  Hint Constructors nc_ms.
+
+  Lemma normalize_comp_fsim_sk1':
+    forward_simulation 1 1 (comp_semantics' L1 L2 sk)
+                       (comp_semantics' (L1 o 1) (1 o L2) sk).
+  Proof.
+    constructor.
+    eapply Forward_simulation with
+      (ltof _ (fun _ => O)) (fun _ _ _ x s1 s2 => x = s1 /\ nc_ms s1 s2).
+    reflexivity. firstorder. 2: apply well_founded_ltof.
+    intros se ? [] [] Hse.
+    eapply forward_simulation_plus.
+    - intros. inv H. inv H0.
+      eexists. split; eauto.
+      repeat constructor; eauto.
+    - intros. inv H0. inv H.
+      exists r1. split; repeat constructor; eauto.
+    - intros. inv H0. inv H. exists tt.
+      exists q1. repeat split; eauto.
+      intros. inv H. inv H0.
+      eexists. split; repeat constructor; eauto.
+    - intros. inv H0.
+      + inv H.
+        * eexists. split; eauto.
+          apply plus_one. apply step1. apply step1. assumption.
+        * eexists; split; eauto.
+          eapply plus_three.
+          apply step1. eapply step_push; try constructor; eauto.
+          eapply step_push; repeat constructor; eauto.
+          apply step2. eapply step_push; try constructor; eauto.
+          reflexivity. eauto.
+      + inv H.
+        * eexists. split; eauto.
+          apply plus_one. apply step2. apply step2. eassumption.
+          eauto.
+        * eexists. split; eauto.
+          eapply plus_three.
+          apply step2. eapply step_pop; try constructor; eauto.
+          eapply step_pop; repeat constructor; eauto.
+          apply step1. eapply step_pop; try constructor; eauto.
+          reflexivity.
+  Qed.
+
+  Lemma normalize_comp_fsim_sk1:
+    forward_simulation 1 1 (normalize_sem (comp_semantics' L1 L2 sk))
+                       (comp_semantics' (normalize_sem L1) (normalize_sem L2) sk).
+  Proof.
+    etransitivity. 2: apply assoc1.
+    unfold normalize_sem. unfold left_comp_id.
+    eapply categorical_compose_simulation'. reflexivity.
+    etransitivity. 2: apply assoc2.
+    etransitivity. 2: apply assoc2.
+    eapply categorical_compose_simulation'. 2: reflexivity.
+    etransitivity. 2: apply assoc1.
+    apply normalize_comp_fsim_sk1'.
+    all: cbn; (apply Linking.linkorder_refl || apply id_skel_order).
+    Unshelve. apply sk.
+  Qed.
+
+  Definition cn_measure (s: state (comp_semantics' (L1 o 1) (1 o L2) sk)) :=
+    match s with
+    | st1 _ _ (st1 _ _ s) => 3%nat
+    | st1 _ _ (st2 _ _ s (st_q _)) => 2%nat
+    | st2 _ _ (st2 _ _ s (st_q _)) (st1 _ _ (st_q _)) => 1%nat
+    | st2 _ _ (st2 _ _ _ (st_q _)) (st2 _ _ (st_q _) _) => 6%nat
+    | st2 _ _ (st2 _ _ s (st_q _)) (st1 _ _ (st_r _)) => 5%nat
+    | st1 _ _ (st2 _ _ s (st_r _)) => 4%nat
+    | _ => 0%nat
+    end.
+  Inductive cn_ms se: state (comp_semantics' (L1 o 1) (1 o L2) sk) ->
+                      state (comp_semantics' L1 L2 sk) -> Prop :=
+  | cn_ms1 s:
+    cn_ms se (st1 (L1 o 1) _ (st1 L1 _ s))
+          (st1 L1 _ s)
+  | cn_ms2 s1 s2 q:
+    cn_ms se (st2 (L1 o 1) (1 o L2) (st2 L1 1 s1 (st_q q)) (st2 1 L2 (st_q q) s2))
+          (st2 L1 L2 s1 s2)
+  | cn_ms3 s q:
+    at_external (L1 se) s q ->
+    cn_ms se (st1 (L1 o 1) _ (st2 L1 1 s (st_q q)))
+          (st1 L1 _ s)
+  | cn_ms4 s q:
+    at_external (L1 se) s q ->
+    cn_ms se (st2 (L1 o 1) (1 o L2) (st2 L1 1 s (st_q q)) (st1 1 _ (st_q q)))
+          (st1 L1 _ s)
+  | cn_ms5 s1 s2 q r:
+    final_state (L2 se) s2 r ->
+    cn_ms se (st2 (L1 o 1) (1 o L2) (st2 L1 1 s1 (st_q q)) (st1 1 _ (st_r r)))
+          (st2 L1 L2 s1 s2)
+  | cn_ms6 s1 s2 r:
+    final_state (L2 se) s2 r ->
+    cn_ms se (st1 (L1 o 1) _ (st2 L1 1 s1 (st_r r)))
+          (st2 L1 L2 s1 s2).
+  Hint Constructors cn_ms.
+
+  Lemma normalize_comp_fsim_sk2':
+    forward_simulation 1 1 (comp_semantics' (L1 o 1) (1 o L2) sk)
+                       (comp_semantics' L1 L2 sk).
+  Proof.
+    constructor.
+    eapply Forward_simulation
+      with (fsim_order := (ltof _ cn_measure))
+           (fsim_match_states := fun _ se _ i s1 s2 =>
+                                   i = s1 /\ cn_ms se s1 s2).
+    reflexivity. firstorder. 2: apply well_founded_ltof.
+    intros se ? [] [] Hse.
+    eapply forward_simulation_opt.
+    - intros. inv H. inv H0. inv H.
+      eexists. split; eauto. constructor. assumption.
+    - intros. inv H0. inv H1. inv H.
+      eexists. split; eauto.
+      constructor. eassumption. constructor.
+    - intros. exists tt. inv H0. inv H1. inv H.
+      eexists. repeat split; eauto.
+      intros. inv H. inv H1. inv H5.
+      eexists. split; eauto. constructor. assumption.
+    - unfold left_comp_id, right_comp_id; intros.
+      inv H0; repeat (inv_comp || inv_id).
+      + left. eexists. split; eauto.
+        apply step1. assumption.
+      + (* 2 < 3 *)
+        right. repeat split; eauto.
+      + left. eexists. split; eauto.
+        apply step2. assumption.
+      + (* 5 < 6 *)
+        right. repeat split; eauto.
+      + (* 1 < 2 *)
+        right. repeat split; eauto.
+      + left. eexists. split; eauto.
+        eapply step_push; eauto.
+      + (* 4 < 5 *)
+        right. repeat split; eauto.
+      + left. eexists. split; eauto.
+        eapply step_pop; eauto.
+  Qed.
+
+  Lemma normalize_comp_fsim_sk2:
+    forward_simulation 1 1 (comp_semantics' (normalize_sem L1) (normalize_sem L2) sk)
+                       (normalize_sem (comp_semantics' L1 L2 sk)).
+  Proof.
+    etransitivity. apply assoc2.
+    eapply categorical_compose_simulation'. reflexivity.
+    etransitivity. apply assoc1.
+    etransitivity. apply assoc1.
+    eapply categorical_compose_simulation'. 2: reflexivity.
+    etransitivity. apply assoc2.
+    apply normalize_comp_fsim_sk2'.
+    all: cbn; (apply Linking.linkorder_refl || apply id_skel_order).
+    Unshelve. apply sk.
+  Qed.
+
+End NORMALIZE_COMP.
